Tests/package.lean
@@ -1,3 +1,4 @@
 
+import «Tests».EquivIsoDemo
 import «Tests».DOT.Sanity
 import «Tests».DTLC.package
